examples/containers/module-edits/Data/IntSet/Internal/midamble.v
@@ -1,45 +1,37 @@
 Require Coq.ZArith.Zcomplements.
+Require Import Coq.ZArith.Zpower.
 Require Import Coq.Numbers.BinNums.
 
-Definition shiftLL (n: Nat) (s : BinInt.Z) : Nat :=
-	Coq.NArith.BinNat.N.shiftl n (Coq.ZArith.BinInt.Z.to_N s).
-Definition shiftRL (n: Nat) (s : BinInt.Z) : Nat :=
-	Coq.NArith.BinNat.N.shiftr n (Coq.ZArith.BinInt.Z.to_N s).
-
-Definition highestBitMask (n: Nat) : Nat := Coq.NArith.BinNat.N.pow 2 (Coq.NArith.BinNat.N.log2 n).
-
 Require Import NArith.
-Definition bit_N := shiftLL 1%N.
+Definition bit_N := fun s => Coq.NArith.BinNat.N.shiftl 1%N (Coq.ZArith.BinInt.Z.to_N s).
 
 Definition popCount_N : N -> Z := unsafeFix (fun popCount x =>
   if Coq.NArith.BinNat.N.eqb x 0
   then 0%Z
   else Coq.ZArith.BinInt.Z.succ (popCount (Coq.NArith.BinNat.N.ldiff x (Coq.NArith.BinNat.N.pow 2 (Coq.NArith.BinNat.N.log2 x))))).
 
-Definition bitCount_N (a : GHC.Num.Int) (x : N) := a GHC.Num.+ (popCount_N x).
-
 Instance Bits__N : Data.Bits.Bits N :=  {
-  op_zizazi__ := N.land ;
-  op_zizbzi__ := N.lor ;
-  bit := bit_N;
-  bitSizeMaybe := fun _ => None ;
-  clearBit := fun n i => N.clearbit n (Coq.ZArith.BinInt.Z.to_N i) ;
-  complement := fun _ => 0%N  ; (* Not legally possible with N *)
+  op_zizazi__   := N.land ;
+  op_zizbzi__   := N.lor ;
+  bit           := bit_N;
+  bitSizeMaybe  := fun _ => None ;
+  clearBit      := fun n i => N.clearbit n (Coq.ZArith.BinInt.Z.to_N i) ;
+  complement    := fun _ => 0%N  ; (* Not legally possible with N *)
   complementBit := fun x i => N.lxor x (bit_N i) ;
-  isSigned := fun x => true ;
-  popCount := popCount_N ;
-  rotate := shiftLL;
-  rotateL := shiftRL;
-  rotateR := shiftRL;
-  setBit := fun x i => N.lor x (bit_N i);
-  shift := shiftLL;
-  shiftL := shiftLL;
-  shiftR := shiftRL;
-  testBit := fun x i => N.testbit x (Coq.ZArith.BinInt.Z.to_N i);
-  unsafeShiftL := shiftLL;
-  unsafeShiftR := shiftRL;
-  xor := N.lxor;
-  zeroBits := 0;
+  isSigned      := fun x => true ;
+  popCount      := popCount_N ;
+  rotate        := fun n s => Coq.NArith.BinNat.N.shiftl n (Coq.ZArith.BinInt.Z.to_N s);
+  rotateL       := fun n s => Coq.NArith.BinNat.N.shiftl n (Coq.ZArith.BinInt.Z.to_N s);
+  rotateR       := fun n s => Coq.NArith.BinNat.N.shiftr n (Coq.ZArith.BinInt.Z.to_N s);
+  setBit        := fun x i => N.lor x (bit_N i);
+  shift         := fun n s => Coq.NArith.BinNat.N.shiftl n (Coq.ZArith.BinInt.Z.to_N s);
+  shiftL        := fun n s => Coq.NArith.BinNat.N.shiftl n (Coq.ZArith.BinInt.Z.to_N s);
+  shiftR        := fun n s => Coq.NArith.BinNat.N.shiftr n (Coq.ZArith.BinInt.Z.to_N s);
+  testBit       := fun x i => N.testbit x (Coq.ZArith.BinInt.Z.to_N i);
+  unsafeShiftL  := fun n s => Coq.NArith.BinNat.N.shiftl n (Coq.ZArith.BinInt.Z.to_N s);
+  unsafeShiftR  := fun n s => Coq.NArith.BinNat.N.shiftr n (Coq.ZArith.BinInt.Z.to_N s);
+  xor           := N.lxor;
+  zeroBits      := 0;
 }.
 
 
@@ -58,3 +50,76 @@ Ltac termination_by_omega :=
 
 (* Z.ones 6 = 64-1 *)
 Definition suffixBitMask : GHC.Num.Int := (Coq.ZArith.BinInt.Z.ones 6)%Z.
+
+
+(** ** [Int64] *)
+
+Definition shiftLL (n: Int64.int) (s : BinInt.Z) : Int64.int :=
+	Int64.shl n (Int64.repr s).
+Definition shiftRL (n: Int64.int) (s : BinInt.Z) : Int64.int :=
+	Int64.shr n (Int64.repr s).
+
+(*  indexOfTheOnlyBit uses pointers and ugly stuff *)
+Definition indexOfTheOnlyBit : Int64.int -> BinInt.Z :=
+ fun x => match Int64.is_power2 x with
+	| Some i => Int64.unsigned i
+	| None => 0%Z
+        end.
+
+Fixpoint last_or_0 (l : list Z) : Z := match l with
+  | nil        => 0
+  | cons i nil => i
+  | cons i xs  => last_or_0 xs
+  end.
+
+Definition highestBitPos (x: Int64.int) : Z :=
+  last_or_0 (Int64.Z_one_bits Int64.wordsize (Int64.unsigned x) 0).
+
+Definition highestBitMask (x: Int64.int) : Int64.int :=
+  Int64.repr (two_p (highestBitPos x)).
+
+Definition popCount_64 (x : Int64.int) :=
+  BinInt.Z.of_nat (length (Int64.Z_one_bits Int64.wordsize (Int64.unsigned x) 0)).
+
+Definition bit_64 (x : Z) := Int64.repr (two_p x).
+
+(* We treat the Int64.int as unsigned here *)
+Instance Num__Int64 : GHC.Num.Num Int64.int  := {
+    op_zp__ := Int64.add;
+    op_zm__ := Int64.sub;
+    op_zt__ := Int64.mul;
+    abs := id;
+    fromInteger := Int64.repr;
+    negate := Int64.neg;
+    signum := id;
+}.
+
+Instance Eq__Int64 : GHC.Base.Eq_ Int64.int  := fun _ k => k {|
+    GHC.Base.op_zeze____ := Int64.eq;
+    GHC.Base.op_zsze____ := (fun x y => Int64.eq x y);
+|}.
+
+Instance Bits__Int64 : Data.Bits.Bits Int64.int :=  {
+  op_zizazi__   := Int64.and ;
+  op_zizbzi__   := Int64.or ;
+  bit           := bit_64;
+  bitSizeMaybe  := fun _ => None ;
+  clearBit      := fun n i => Int64.and n (bit_64 i);
+  complement    := Int64.not;
+  complementBit := fun x i => Int64.xor x (bit_64 i);
+  isSigned      := fun x => true;
+  popCount      := popCount_64 ;
+  rotate        := fun n s => Int64.shl  n (Int64.repr s);
+  rotateL       := fun n s => Int64.shl  n (Int64.repr s);
+  rotateR       := fun n s => Int64.shru n (Int64.repr s);
+  setBit        := fun x i => Int64.or x (bit_64 i);
+  shift         := fun n s => Int64.shl  n (Int64.repr s);
+  shiftL        := fun n s => Int64.shl  n (Int64.repr s);
+  shiftR        := fun n s => Int64.shru n (Int64.repr s);
+  testBit       := fun x i => Int64.testbit x i;
+  unsafeShiftL  := fun n s => Int64.shl  n (Int64.repr s);
+  unsafeShiftR  := fun n s => Int64.shru n (Int64.repr s);
+  xor           := Int64.xor;
+  zeroBits      := Int64.zero;
+}.
+
